theories/FullQuote.v
@@ -14,17 +14,31 @@ Import ListNotations.
 
 Inductive assocn (A : Type) :=
 | emptyn
-| aconsn (key : string) (n : nat) (data : A) (t : assocn A).
+| aconsn (key : kername) (n : nat) (data : A) (t : assocn A).
 
 Arguments emptyn {_}.
 Arguments aconsn {_} _ _ _.
 
-Fixpoint assocn_at {A} (key : string) (n : nat) (t : assocn A) {struct t}
+Fixpoint assocn_at {A} (key : kername) (n : nat) (t : assocn A) {struct t}
   : option A :=
   match t with
   | emptyn => None
   | aconsn k m a r =>
-    if (ident_eq key k) && (n =? m) then Some a else assocn_at key n r
+    if (eq_kername key k) && (n =? m) then Some a else assocn_at key n r
+  end.
+
+(* Associative table indexed by kernames *)
+Inductive assock (A : Type) :=
+| emptyk
+| aconsk (key : kername) (data : A) (t : assock A).
+
+Arguments emptyk {_}.
+Arguments aconsk {_} _ _.
+
+Fixpoint assock_at {A} (key : kername) (t : assock A) {struct t} : option A :=
+  match t with
+  | emptyk => None
+  | aconsk k a r => if eq_kername key k then Some a else assock_at key r
   end.
 
 Inductive fq_error :=
@@ -32,9 +46,9 @@ Inductive fq_error :=
 | NotHandled (t : term)
 | TypingError (msg : string) (e : type_error) (Γ : context) (t : term)
 | WrongType (wanted : string) (got : term)
-| UnknownInductive (id : string)
-| UnknownConst (id : string)
-| UnknownConstruct (id : string) (n : nat)
+| UnknownInductive (id : kername)
+| UnknownConst (id : kername)
+| UnknownConstruct (id : kername) (n : nat)
 .
 
 Inductive fq_result A :=
@@ -70,8 +84,10 @@ Open Scope string_scope.
 
 Existing Instance default_fuel.
 
+Definition an (a : aname) : name := binder_name a.
+
 Fixpoint fullquote (fuel : nat) (Σ : global_env) (G : universes_graph)
-  (Γ : context) (t : term) (indt : assoc sterm) (constt : assoc sterm)
+  (Γ : context) (t : term) (indt : assock sterm) (constt : assock sterm)
   (cot : assocn sterm) {struct fuel}
   : fq_result sterm :=
   match fuel with
@@ -83,25 +99,54 @@ Fixpoint fullquote (fuel : nat) (Σ : global_env) (G : universes_graph)
     | tProd nx A B =>
       A' <- fullquote fuel Σ G Γ A indt constt cot ;;
       B' <- fullquote fuel Σ G (Γ ,, vass nx A) B indt constt cot ;;
-      ret (sProd nx A' B')
+      ret (sProd (an nx) A' B')
     | tLambda nx A t =>
       match infer_hnf Σ G (Γ ,, vass nx A) t with
       | Checked B =>
         A' <- fullquote fuel Σ G Γ A indt constt cot ;;
         B' <- fullquote fuel Σ G (Γ ,, vass nx A) B indt constt cot ;;
         t' <- fullquote fuel Σ G (Γ ,, vass nx A) t indt constt cot ;;
-        ret (sLambda nx A' B' t')
+        ret (sLambda (an nx) A' B' t')
       | TypeError e => raise (TypingError "Lambda" e (Γ ,, vass nx A) t)
       end
-    | tApp (tConst "Translation.Quotes.candidate" []) [ _ ; _ ; t ] =>
-      fullquote fuel Σ G Γ t indt constt cot
+    | tApp u l =>
+      match u, l with
+      | tConst id ui, [ A ; B ; t ] =>
+        if eq_kername id (MPfile ["Quotes"; "Translation"], "candidate")%core
+        then fullquote fuel Σ G Γ t indt constt cot
+        else fullquote fuel Σ G Γ (tApp (tApp u [ A ]) [ B ; t ]) indt constt cot
+      | tInd {| inductive_mind := id ; inductive_ind := 0 |} ui, [ A ; x ; y ] =>
+        if eq_kername id (MPfile ["Logic"; "Init"; "Coq"], "eq")%core
+        then
+          A' <- fullquote fuel Σ G Γ A indt constt cot ;;
+          x' <- fullquote fuel Σ G Γ x indt constt cot ;;
+          y' <- fullquote fuel Σ G Γ y indt constt cot ;;
+          ret (sEq A' x' y')
+        else fullquote fuel Σ G Γ (tApp (tApp u [ A ]) [ x ; y ]) indt constt cot
+      | u, [ v ] =>
+        match infer_hnf Σ G Γ u with
+        | Checked (tProd nx A B) =>
+          u' <- fullquote fuel Σ G Γ u indt constt cot ;;
+          A' <- fullquote fuel Σ G Γ A indt constt cot ;;
+          B' <- fullquote fuel Σ G (Γ ,, vass nx A) B indt constt cot ;;
+          v' <- fullquote fuel Σ G Γ v indt constt cot ;;
+          ret (sApp u' A' B' v')
+        | Checked T => raise (WrongType "Prod" T)
+        | TypeError e => raise (TypingError "App1" e Γ u)
+        end
+      | u, v :: l =>
+        fullquote fuel Σ G Γ (tApp (tApp u [ v ]) l) indt constt cot
+      | u, [] =>
+        fullquote fuel Σ G Γ u indt constt cot
+      (* | _ => raise (NotHandled t) *)
+      end
     | tInd {| inductive_mind := id ; inductive_ind := _ |} [] =>
-      match assoc_at id indt with
+      match assock_at id indt with
       | Some t => ret t
       | None => raise (UnknownInductive id)
       end
     | tConst id [] =>
-      match assoc_at id constt with
+      match assock_at id constt with
       | Some t => ret t
       | None => raise (UnknownConst id)
       end
@@ -110,26 +155,6 @@ Fixpoint fullquote (fuel : nat) (Σ : global_env) (G : universes_graph)
       | Some t => ret t
       | None => raise (UnknownConstruct id n)
       end
-    | tApp (tInd {| inductive_mind := "Coq.Init.Logic.eq"; inductive_ind := 0 |} []) [ A ; u ; v ] =>
-      A' <- fullquote fuel Σ G Γ A indt constt cot ;;
-      u' <- fullquote fuel Σ G Γ u indt constt cot ;;
-      v' <- fullquote fuel Σ G Γ v indt constt cot ;;
-      ret (sEq A' u' v')
-    | tApp u [] =>
-      fullquote fuel Σ G Γ u indt constt cot
-    | tApp u [ v ] =>
-      match infer_hnf Σ G Γ u with
-      | Checked (tProd nx A B) =>
-        u' <- fullquote fuel Σ G Γ u indt constt cot ;;
-        A' <- fullquote fuel Σ G Γ A indt constt cot ;;
-        B' <- fullquote fuel Σ G (Γ ,, vass nx A) B indt constt cot ;;
-        v' <- fullquote fuel Σ G Γ v indt constt cot ;;
-        ret (sApp u' A' B' v')
-      | Checked T => raise (WrongType "Prod" T)
-      | TypeError e => raise (TypingError "App1" e Γ u)
-      end
-    | tApp u (v :: l) =>
-      fullquote fuel Σ G Γ (tApp (tApp u [ v ]) l) indt constt cot
     | tCast t _ _ => fullquote fuel Σ G Γ t indt constt cot
     | _ => raise (NotHandled t)
     end
